src/program_proof/rsm/distx/action.v
@@ -6,16 +6,31 @@ From Perennial.program_proof.rsm.distx Require Import base.
 Definition head_commit (l : list action) (ts : nat) (wrs : dbmap) :=
   head l = Some (ActCommit ts wrs).
 
+Definition head_abort (l : list action) (ts : nat) :=
+  head l = Some (ActAbort ts).
+
 Definition head_read (l : list action) (ts : nat) (key : dbkey) :=
   head l = Some (ActRead ts key).
 
-Definition no_commit (l : list action) (tid : nat) :=
-  ∀ wrs, ActCommit tid wrs ∉ l.
+Definition no_commit_abort (l : list action) (tid : nat) :=
+  ActAbort tid ∉ l ∧ ∀ wrs, ActCommit tid wrs ∉ l.
+
+Definition first_abort (l : list action) (ts : nat) :=
+  ∃ lp ls,
+    l = lp ++ ls ∧
+    no_commit_abort lp ts ∧
+    head ls = Some (ActAbort ts).
+
+Definition first_commit (l lp ls : list action) (ts : nat) (wrs : dbmap) :=
+  l = lp ++ ls ∧
+  no_commit_abort lp ts ∧
+  head ls = Some (ActCommit ts wrs).
 
 Definition compatible (ts : nat) (wrs : dbmap) (a : action) :=
   match a with
   | ActCommit tsa wrsa => (tsa < ts)%nat ∨ (dom wrs) ∩ (dom wrsa) = ∅
   | ActRead tsa key => (tsa ≤ ts)%nat ∨ key ∉ (dom wrs)
+  | _ => True
   end.
 
 #[local]
@@ -44,11 +59,6 @@ timestamp [ts] is [ActCommit ts wrs]". However, [first_commit_incompatible]
 needs access to the first part of [l] (i.e., the one without any commit action
 of timestamp [ts], so we expose [lp] and [ls] as well. *)
 
-Definition first_commit (l lp ls : list action) (ts : nat) (wrs : dbmap) :=
-  l = lp ++ ls ∧
-  no_commit lp ts ∧
-  head ls = Some (ActCommit ts wrs).
-
 Definition first_commit_incompatible (l1 l2 : list action) (ts : nat) (wrs : dbmap) :=
   ∃ lp ls,
     first_commit l2 lp ls ts wrs ∧
@@ -59,108 +69,156 @@ Definition first_commit_compatible (l : list action) (ts : nat) (wrs : dbmap) :=
     first_commit l lp ls ts wrs ∧
     compatible_all lp ts wrs.
 
-Fixpoint find_max_prefix_before_commit (ts : nat) (lp ls : list action) : (list action * list action) :=
-  match ls with
-  | [] => (lp, ls)
-  | hd :: tl => match hd with
-              | ActCommit tshd _ => if decide (tshd = ts)
-                                   then (lp, ls)
-                                   else find_max_prefix_before_commit ts (lp ++ [hd]) tl
-              | ActRead _ _ => find_max_prefix_before_commit ts (lp ++ [hd]) tl
-              end
+Definition is_commit_abort_of_ts (ts : nat) act :=
+  match act with
+  | ActCommit tid _ => tid = ts
+  | ActAbort tid => tid = ts
+  | _ => False
   end.
 
-Lemma find_max_prefix_before_commit_spec ts lp ls :
+Lemma is_commit_abort_of_ts_spec ts act :
+  is_commit_abort_of_ts ts act ->
+  act = ActAbort ts ∨ ∃ wrs, act = ActCommit ts wrs.
+Proof.
+  intros Hca.
+  destruct act; last done; rewrite Hca.
+  - right. by eauto.
+  - by left.
+Qed.
+
+#[local]
+Instance is_commit_abort_of_ts_dec ts a : Decision (is_commit_abort_of_ts ts a).
+Proof. destruct a; simpl; apply _. Defined.
+
+Fixpoint find_max_prefix_before_commit_abort
+  (ts : nat) (lp ls : list action) : (list action * list action) :=
+  match ls with
+  | [] => (lp, ls)
+  | hd :: tl => if decide (is_commit_abort_of_ts ts hd)
+              then (lp, ls)
+              else find_max_prefix_before_commit_abort ts (lp ++ [hd]) tl
+  end.
+
+Lemma find_max_prefix_before_commit_abort_spec ts lp ls :
   ∃ ls1 ls2,
-    find_max_prefix_before_commit ts lp ls = (lp ++ ls1, ls2) ∧
+    find_max_prefix_before_commit_abort ts lp ls = (lp ++ ls1, ls2) ∧
     ls = ls1 ++ ls2 ∧
-    no_commit ls1 ts ∧
-    (ls2 = [] ∨ ∃ wrs, head ls2 = Some (ActCommit ts wrs)).
+    no_commit_abort ls1 ts ∧
+    match head ls2 with
+    | Some a => is_commit_abort_of_ts ts a
+    | _ => True
+    end.
+    (* (ls2 = [] ∨ is_commit_abort_of_ts ts (head ls2)). *)
 Proof.
   generalize dependent lp.
+  rewrite /no_commit_abort.
   induction ls as [| a ls IH]; intros lp; simpl.
   { exists [], [].
     split; first by rewrite app_nil_r.
     split; first done.
-    split.
-    { rewrite /no_commit. set_solver. }
-    by left.
+    split; last done.
+    rewrite /no_commit_abort. set_solver.
   }
-  destruct a as [tsa wrs | tsa key] eqn:Ha; rewrite -Ha; last first.
-  { destruct (IH (lp ++ [a])) as (ls1 & ls2 & Heq & Hls2 & Hnc & Hhead).
+  case_decide as Ha.
+  - destruct (IH (lp ++ [a])) as (ls1 & ls2 & Heq & Hls2 & Hnca & Hhead).
+    exists [], (a :: ls).
+    split; first by rewrite app_nil_r.
+    split; set_solver.
+  - destruct (IH (lp ++ [a])) as (ls1 & ls2 & Heq & Hls2 & Hnca & Hhead).
     exists ([a] ++ ls1), ls2.
     split; first by rewrite app_assoc Heq.
-    split; first set_solver.
-    split.
-    { intros wrsa.
-      rewrite not_elem_of_app.
-      split; [set_solver | done].
-    }
-    done.
-  }
-  case_decide as Htsa; last first.
-  { destruct (IH (lp ++ [a])) as (ls1 & ls2 & Heq & Hls2 & Hnc & Hhead).
-    exists ([a] ++ ls1), ls2.
-    split; first by rewrite app_assoc Heq.
-    split; first set_solver.
-    split.
-    { intros wrsa.
-      rewrite not_elem_of_app.
-      split; [set_solver | done].
-    }
-    done.
-  }
-  exists [], (a :: ls).
-  split; first by rewrite app_nil_r.
-  split; first by rewrite app_nil_l.
-  split.
-  { rewrite /no_commit. set_solver. }
-  right.
-  rewrite Ha Htsa.
-  by eauto.
+    split; set_solver.
 Qed.
 
 Inductive tcform :=
-(* no commit in the entire list of actions *)
-| NC
-(* first commit incompatible with some previous actions *)
+(* no commit or abort in the entire list of actions *)
+| NCA
+(* first action is abort *)
+| FA
+(* first action is commit and it's incompatible with some previous actions *)
 | FCI (wrs : dbmap)
-(* first commit compatible with some previous actions *)
+(* first action is commit and it's compatible with some previous actions *)
 | FCC (wrs : dbmap).
 
 Definition peek (l : list action) (ts : nat) : tcform :=
-  let (lp, ls) := find_max_prefix_before_commit ts [] l in
+  let (lp, ls) := find_max_prefix_before_commit_abort ts [] l in
   match head ls with
-  | None => NC
+  | None => NCA
   | Some a => match a with
              | ActCommit _ wrs => if decide (compatible_all lp ts wrs)
                                  then FCC wrs
                                  else FCI wrs
-             | _ => NC (* impossible case *)
+             | _ => FA
              end
   end.
 
-Theorem peek_spec l ts :
-  match peek l ts with
-  | NC => no_commit l ts
-  | FCI wrs => first_commit_incompatible [] l ts wrs
-  | FCC wrs => first_commit_compatible l ts wrs
+Definition conflict_cases
+  (past future : list action) (ts : nat) (form : tcform) :=
+  match form with
+  | NCA => no_commit_abort future ts
+  | FA => first_abort future ts
+  | FCI wrs => first_commit_incompatible past future ts wrs
+  | FCC wrs => first_commit_compatible future ts wrs
   end.
+
+Theorem peek_spec l ts :
+  conflict_cases [] l ts (peek l ts).
 Proof.
   unfold peek.
-  destruct (find_max_prefix_before_commit_spec ts [] l) as (lp & ls & -> & Hl & Hnc & Hls).
-  destruct Hls as [Hls | [wrs Hls]].
-  { subst ls. by rewrite /= Hl app_nil_r. }
-  rewrite Hls.
+  destruct (find_max_prefix_before_commit_abort_spec ts [] l) as (lp & ls & -> & Hl & Hnca & Hls).
+  destruct (head ls) as [a |] eqn:Hhead; last first.
+  { rewrite head_None in Hhead. subst ls. by rewrite /= Hl app_nil_r. }
+  apply is_commit_abort_of_ts_spec in Hls.
+  destruct Hls as [-> | [wrs ->]].
+  { by exists lp, ls. }
   case_decide as Hcomp.
   { by exists lp, ls. }
   { exists lp, ls. by rewrite -not_compatible_all_incompatible_exists. }
 Qed.
 
-Lemma no_commit_inv_tail_future future ts :
-  no_commit future ts ->
-  no_commit (tail future) ts.
-Proof. intros Hnc wrs. by apply not_elem_of_tail. Qed.
+Lemma first_commit_head_abort future lp ls ts wrs :
+  first_commit future lp ls ts wrs ->
+  head_abort future ts ->
+  False.
+Proof.
+  intros (Happ & [Hna _] & Hhead) Hha.
+  destruct lp as [| x l]; last first.
+  { rewrite Happ /head_abort /= in Hha.
+    inv Hha.
+    set_solver.
+  }
+  rewrite Happ /= /head_abort Hhead in Hha.
+  by inv Hha.
+Qed.
+
+Lemma no_commit_abort_inv_tail_future future ts :
+  no_commit_abort future ts ->
+  no_commit_abort (tail future) ts.
+Proof.
+  intros [Hna Hnca].
+  split.
+  - by apply not_elem_of_tail.
+  - intros wrs. by apply not_elem_of_tail.
+Qed.
+
+Lemma first_abort_inv_tail_future future ts a :
+  a ≠ ActAbort ts ->
+  head future = Some a ->
+  first_abort future ts ->
+  first_abort (tail future) ts.
+Proof.
+  intros Hne Hhead (lp & ls & (Happ & Hnca & Hheadls)).
+  assert (Hnnil : lp ≠ nil).
+  { intros Hlp. subst lp.
+    simpl in Happ. subst ls.
+    rewrite Hhead in Hheadls.
+    inv Hheadls.
+  }
+  exists (tail lp), ls.
+  split.
+  { rewrite Happ. apply tail_app_l, Hnnil. }
+  by split; first apply no_commit_abort_inv_tail_future.
+Qed.
 
 Lemma first_commit_incompatible_inv_snoc_past_tail_future past future ts wrs a :
   a ≠ ActCommit ts wrs ->
@@ -168,7 +226,7 @@ Lemma first_commit_incompatible_inv_snoc_past_tail_future past future ts wrs a :
   first_commit_incompatible past future ts wrs ->
   first_commit_incompatible (past ++ [a]) (tail future) ts wrs.
 Proof.
-  intros Hne Hhead (lp & ls & (Happ & Hnc & Hheadls) & Hincomp).
+  intros Hne Hhead (lp & ls & (Happ & Hnca & Hheadls) & Hincomp).
   assert (Hnnil : lp ≠ nil).
   { intros Hlp. subst lp.
     simpl in Happ. subst ls.
@@ -179,7 +237,7 @@ Proof.
   split.
   { split.
     { rewrite Happ. apply tail_app_l, Hnnil. }
-    by split; first apply no_commit_inv_tail_future.
+    by split; first apply no_commit_abort_inv_tail_future.
   }
   rewrite -app_assoc /=.
   replace (_ :: _) with lp; first apply Hincomp.
@@ -191,13 +249,12 @@ Proof.
   by apply prefix_app_r.
 Qed.
 
-Lemma first_commit_compatible_inv_tail_future future ts wrs a :
-  a ≠ ActCommit ts wrs ->
-  head future = Some a ->
-  first_commit_compatible future ts wrs ->
-  first_commit_compatible (tail future) ts wrs.
+Lemma first_commit_incompatible_inv_tail_future past future ts tshd wrs :
+  head_abort future tshd ->
+  first_commit_incompatible past future ts wrs ->
+  first_commit_incompatible past (tail future) ts wrs.
 Proof.
-  intros Hne Hhead (lp & ls & (Happ & Hnc & Hheadls) & Hincomp).
+  intros Hhead (lp & ls & (Happ & Hnca & Hheadls) & Hincomp).
   assert (Hnnil : lp ≠ nil).
   { intros Hlp. subst lp.
     simpl in Happ. subst ls.
@@ -208,7 +265,40 @@ Proof.
   split.
   { split.
     { rewrite Happ. apply tail_app_l, Hnnil. }
-    by split; first apply no_commit_inv_tail_future.
+    by split; first apply no_commit_abort_inv_tail_future.
+  }
+  revert Hincomp.
+  rewrite /incompatible_exists 2!Exists_app.
+  intros Hincomp.
+  destruct Hincomp as [Hincomp | Hincomp]; first by left.
+  right.
+  destruct lp as [| x t]; first done. simpl.
+  rewrite Exists_cons in Hincomp.
+  destruct Hincomp as [Hincomp | Hincomp]; last done.
+  exfalso.
+  rewrite /head_abort Happ /= in Hhead.
+  inv Hhead.
+  by rewrite /incompatible in Hincomp.
+Qed.
+
+Lemma first_commit_compatible_inv_tail_future future ts wrs a :
+  a ≠ ActCommit ts wrs ->
+  head future = Some a ->
+  first_commit_compatible future ts wrs ->
+  first_commit_compatible (tail future) ts wrs.
+Proof.
+  intros Hne Hhead (lp & ls & (Happ & Hnca & Hheadls) & Hincomp).
+  assert (Hnnil : lp ≠ nil).
+  { intros Hlp. subst lp.
+    simpl in Happ. subst ls.
+    rewrite Hhead in Hheadls.
+    inv Hheadls.
+  }
+  exists (tail lp), ls.
+  split.
+  { split.
+    { rewrite Happ. apply tail_app_l, Hnnil. }
+    by split; first apply no_commit_abort_inv_tail_future.
   }
   by apply Forall_tail.
 Qed.
