src/program_proof/rsm/distx/inv_txnsys.v
@@ -7,14 +7,6 @@ From Perennial.program_proof.rsm.pure Require Import dual_lookup vslice nat.
 Definition conflict_free (future : list action) (tmodcs : gmap nat dbmap) :=
   map_Forall (λ t m, first_commit_compatible future t m) tmodcs.
 
-Definition conflict_cases
-  (past future : list action) (ts : nat) (form : tcform) :=
-  match form with
-  | NC => no_commit future ts
-  | FCI wrs => first_commit_incompatible past future ts wrs
-  | FCC wrs => first_commit_compatible future ts wrs
-  end.
-
 Definition conflict_past (past future : list action) (tmodas : gmap nat tcform) :=
   map_Forall (λ t m, conflict_cases past future t m) tmodas.
 
@@ -53,14 +45,14 @@ Definition cmtxn_in_past (past : list action) (resm : gmap nat txnres) :=
   map_Forall (λ t m, ActCommit t m ∈ past) (resm_to_tmods resm).
 
 Lemma resm_to_tmods_insert_aborted resm ts :
-  resm !! ts = None ->
+  resm !! ts = None ∨ resm !! ts = Some ResAborted ->
   resm_to_tmods (<[ts := ResAborted]> resm) = resm_to_tmods resm.
 Proof.
   intros Hresm.
   apply map_eq. intros tsx.
   rewrite 2!lookup_omap.
   destruct (decide (tsx = ts)) as [-> | Hne]; last by rewrite lookup_insert_ne.
-  by rewrite lookup_insert Hresm.
+  by destruct Hresm as [Hresm | Hresm]; rewrite lookup_insert Hresm.
 Qed.
 
 Lemma resm_to_tmods_insert_committed resm ts wrs :
@@ -127,6 +119,11 @@ Definition incorrect_fcc Qr form :=
   |_ => True
   end.
 
+#[global]
+Instance incorrect_fcc_decision Qr {H : ∀ m, Decision (Qr m)} form :
+  Decision (incorrect_fcc Qr form).
+Proof. destruct form; apply _. Defined.
+
 Section inv.
   Context `{!distx_ghostG Σ}.
   (* TODO: remove this once we have real defintions for resources. *)
@@ -141,12 +138,61 @@ Section inv.
     "Hwcmts" ∷ ([∗ set] tid ∈ wcmts, tids_excl_frag γ tid) ∗
     "Hwabts" ∷ ([∗ set] tid ∈ wabts, tids_excl_frag γ tid) ∗
     "Hcmts"  ∷ ([∗ set] tid ∈ cmts, tids_excl_frag γ tid) ∗
-    "%Hfate" ∷ ⌜set_Forall (λ tid, tid ∈ cmts ∨ tid ∈ wabts ∨ tid ∈ wcmts) tids⌝.
+    "%Hfate" ∷ ⌜set_Forall (λ tid, tid ∈ dom resm ∨ tid ∈ wabts ∨ tid ∈ wcmts) tids⌝.
+
+  Lemma elem_of_tmodcs_partitioned_tids γ tids tmodcs tmodas resm tid :
+    tid ∈ dom tmodcs ->
+    partitioned_tids γ tids tmodcs tmodas resm -∗
+    ⌜tid ∉ dom tmodas ∧ ∀ m, resm !! tid ≠ Some (ResCommitted m)⌝.
+  Proof.
+    iIntros (Hin) "Hpart".
+    iNamed "Hpart".
+    iDestruct (big_sepS_elem_of with "Hwcmts") as "Hexcl"; first apply Hin.
+    iDestruct (tids_excl_not_elem_of with "Hwabts Hexcl") as %Hnotinwa.
+    iDestruct (tids_excl_not_elem_of with "Hcmts Hexcl") as %Hnotinc.
+    iPureIntro.
+    split; first apply Hnotinwa.
+    intros m Hcmt.
+    by rewrite not_elem_of_dom /resm_to_tmods lookup_omap Hcmt /= in Hnotinc.
+  Qed.
+
+  Lemma elem_of_tmodas_partitioned_tids γ tids tmodcs tmodas resm tid :
+    tid ∈ dom tmodas ->
+    partitioned_tids γ tids tmodcs tmodas resm -∗
+    ⌜tid ∉ dom tmodcs ∧ ∀ m, resm !! tid ≠ Some (ResCommitted m)⌝.
+  Proof.
+    iIntros (Hin) "Hpart".
+    iNamed "Hpart".
+    iDestruct (big_sepS_elem_of with "Hwabts") as "Hexcl"; first apply Hin.
+    iDestruct (tids_excl_not_elem_of with "Hwcmts Hexcl") as %Hnotinwc.
+    iDestruct (tids_excl_not_elem_of with "Hcmts Hexcl") as %Hnotinc.
+    iPureIntro.
+    split; first apply Hnotinwc.
+    intros m Hcmt.
+    by rewrite not_elem_of_dom /resm_to_tmods lookup_omap Hcmt /= in Hnotinc.
+  Qed.
+
+  Lemma elem_of_committed_partitioned_tids γ tids tmodcs tmodas resm tid :
+    (∃ m, resm !! tid = Some (ResCommitted m)) ->
+    partitioned_tids γ tids tmodcs tmodas resm -∗
+    ⌜tid ∉ dom tmodcs ∧ tid ∉ dom tmodas⌝.
+  Proof.
+    iIntros (Hm) "Hpart".
+    destruct Hm as [m Hm].
+    iNamed "Hpart".
+    assert (Hin : tid ∈ dom (resm_to_tmods resm)).
+    { by rewrite elem_of_dom /resm_to_tmods lookup_omap Hm /=. }
+    iDestruct (big_sepS_elem_of with "Hcmts") as "Hexcl"; first apply Hin.
+    iDestruct (tids_excl_not_elem_of with "Hwcmts Hexcl") as %Hnotinwc.
+    iDestruct (tids_excl_not_elem_of with "Hwabts Hexcl") as %Hnotinwa.
+    done.
+  Qed.
 
   Definition past_action_witness γ (a : action) : iProp Σ :=
     match a with
     | ActCommit ts wrs => [∗ set] key ∈ dom wrs, hist_cmtd_length_lb γ key (S ts)
     | ActRead ts key => hist_cmtd_length_lb γ key ts
+    | _ => True
     end.
 
   #[global]
@@ -162,18 +208,6 @@ Section inv.
     ∃ gid wrs, txnprep_unprep γ gid ts ∗
                txnwrs_receipt γ ts wrs ∗
                ⌜gid ∈ ptgroups (dom wrs)⌝.
-
-  Lemma all_prepared_some_aborted_false γ ts wrs :
-    all_prepared γ ts wrs -∗
-    some_aborted γ ts -∗
-    ⌜False⌝.
-  Proof.
-    iIntros "[Hwrs Hps] Habt".
-    iDestruct "Habt" as (gid wrsa) "(Hnp & Hwrsa & %Hgid)".
-    iDestruct (txnwrs_receipt_agree with "Hwrs Hwrsa") as %->.
-    iDestruct (big_sepS_elem_of with "Hps") as "Hp"; first apply Hgid.
-    by iDestruct (txnprep_receipt_agree with "Hp Hnp") as %Hcontra.
-  Qed.
 
   Definition correct_wrs γ ts wrs : iProp Σ :=
     ∃ Q, txnpost_receipt γ ts Q ∗ ⌜Q wrs⌝.
@@ -205,17 +239,48 @@ Section inv.
   Definition valid_res γ ts res : iProp Σ :=
     match res with
     | ResCommitted wrs => all_prepared γ ts wrs
-    | ResAborted => some_aborted γ ts
+    | ResAborted => some_aborted γ ts ∨ txnwrs_cancel γ ts
     end.
 
   #[global]
   Instance valid_res_persistent γ ts res :
     Persistent (valid_res γ ts res).
   Proof. destruct res; apply _. Qed.
+  
+  Lemma all_prepared_some_aborted γ ts wrs :
+    all_prepared γ ts wrs -∗
+    some_aborted γ ts -∗
+    False.
+  Proof.
+    iIntros "[Hwrs Hps] Habt".
+    iDestruct "Habt" as (gid wrsa) "(Hnp & Hwrsa & %Hgid)".
+    iDestruct (txnwrs_receipt_agree with "Hwrs Hwrsa") as %->.
+    iDestruct (big_sepS_elem_of with "Hps") as "Hp"; first apply Hgid.
+    by iDestruct (txnprep_receipt_agree with "Hp Hnp") as %Hcontra.
+  Qed.
 
-  Definition txnsys_inv γ : iProp Σ :=
-    ∃ (ts : nat) (tids : gset nat) (future past : list action)
-      (tmodcs : gmap nat dbmap) (tmodas : gmap nat tcform) (posts : gmap nat (dbmap -> Prop))
+  Lemma all_prepared_txnwrs_cancel γ ts wrs :
+    all_prepared γ ts wrs -∗
+    txnwrs_cancel γ ts -∗
+    False.
+  Proof.
+    iIntros "[Hwrs Hps] Hccl".
+    by iDestruct (txnwrs_frag_agree with "Hwrs Hccl") as %Hcontra.
+  Qed.
+
+  Lemma all_prepared_valid_res_aborted γ ts wrs :
+    all_prepared γ ts wrs -∗
+    valid_res γ ts ResAborted -∗
+    False.
+  Proof.
+    iIntros "Hprep [Habt | Hccl]".
+    - iApply (all_prepared_some_aborted with "Hprep Habt").
+    - iApply (all_prepared_txnwrs_cancel with "Hprep Hccl").
+  Qed.
+
+  Definition txnsys_inv γ p : iProp Σ :=
+    ∃ (ts : nat) (tids tidas : gset nat) (future past : list action)
+      (tmods tmodcs : gmap nat dbmap) (tmodas : gmap nat tcform) (posts : gmap nat (dbmap -> Prop))
       (resm : gmap nat txnres) (wrsm : gmap nat (option dbmap)),
       (* global timestamp *)
       "Hts"    ∷ ts_auth γ ts ∗
@@ -224,10 +289,14 @@ Section inv.
       (* exclusive transaction IDs *)
       "Hexcl" ∷ tids_excl_auth γ tids ∗
       "Hpart" ∷ partitioned_tids γ tids tmodcs tmodas resm ∗
+      (* transactions predicted to commit *)
+      "Htidcs" ∷ txns_cmt_auth γ tmods ∗
+      (* transactions predicted to abort *)
+      "Htidas" ∷ txns_abt_auth γ tidas ∗
       (* transaction post-conditions; a better design seems to be moving this out of [txnsys_inv] *)
       "Hpost" ∷ txnpost_auth γ posts ∗
       (* prophecy variable *)
-      "Hproph" ∷ txn_proph γ future ∗
+      "Hproph" ∷ txn_proph γ p future ∗
       (* transaction result map *)
       "Hresm" ∷ txnres_auth γ resm ∗
       (* transaction write set map *)
@@ -244,6 +313,9 @@ Section inv.
       (* past action witnesses *)
       "#Hpas" ∷ ([∗ list] a ∈ past, past_action_witness γ a) ∗
       "%Htsge" ∷ ⌜ge_all ts tids⌝ ∗
+      "%Hintids" ∷ ⌜dom tmods ⊆ tids ∧ tidas ⊆ tids⌝ ∗
+      "%Htidcs" ∷ ⌜map_Forall (λ t m, tmodcs !! t = Some m ∨ resm !! t = Some (ResCommitted m)) tmods⌝ ∗
+      "%Htidas" ∷ ⌜dom tmodas = tidas⌝ ∗
       "%Hdomq" ∷ ⌜dom posts = tids⌝ ∗
       "%Hdomw" ∷ ⌜dom wrsm = tids⌝ ∗
       "%Hcmtxn" ∷ ⌜cmtxn_in_past past resm⌝ ∗
@@ -253,8 +325,8 @@ Section inv.
       "%Hcp"    ∷ ⌜conflict_past past future tmodas⌝.
 
   Definition txnsys_inv_no_future γ future : iProp Σ :=
-    ∃ (ts : nat) (tids : gset nat) (past : list action)
-      (tmodcs : gmap nat dbmap) (tmodas : gmap nat tcform) (posts : gmap nat (dbmap -> Prop))
+    ∃ (ts : nat) (tids tidas : gset nat) (past : list action)
+      (tmods tmodcs : gmap nat dbmap) (tmodas : gmap nat tcform) (posts : gmap nat (dbmap -> Prop))
       (resm : gmap nat txnres) (wrsm : gmap nat (option dbmap)),
       (* global timestamp *)
       "Hts"    ∷ ts_auth γ ts ∗
@@ -263,6 +335,10 @@ Section inv.
       (* exclusive transaction IDs *)
       "Hexcl" ∷ tids_excl_auth γ tids ∗
       "Hpart" ∷ partitioned_tids γ tids tmodcs tmodas resm ∗
+      (* transactions predicted to commit *)
+      "Htidcs" ∷ txns_cmt_auth γ tmods ∗
+      (* transactions predicted to abort *)
+      "Htidas" ∷ txns_abt_auth γ tidas ∗
       (* transaction post-conditions *)
       "Hpost" ∷ txnpost_auth γ posts ∗
       (* transaction result map *)
@@ -281,6 +357,9 @@ Section inv.
       (* past action witnesses *)
       "#Hpas" ∷ ([∗ list] a ∈ past, past_action_witness γ a) ∗
       "%Htsge" ∷ ⌜ge_all ts tids⌝ ∗
+      "%Hintids" ∷ ⌜dom tmods ⊆ tids ∧ tidas ⊆ tids⌝ ∗
+      "%Htidcs" ∷ ⌜map_Forall (λ t m, tmodcs !! t = Some m ∨ resm !! t = Some (ResCommitted m)) tmods⌝ ∗
+      "%Htidas" ∷ ⌜dom tmodas = tidas⌝ ∗
       "%Hdomq" ∷ ⌜dom posts = tids⌝ ∗
       "%Hdomw" ∷ ⌜dom wrsm = tids⌝ ∗
       "%Hcmtxn" ∷ ⌜cmtxn_in_past past resm⌝ ∗
@@ -289,22 +368,34 @@ Section inv.
       "%Hcf"   ∷ ⌜conflict_free future tmodcs⌝ ∗
       "%Hcp"   ∷ ⌜conflict_past past future tmodas⌝.
 
-  Lemma txnsys_inv_extract_future γ :
-    txnsys_inv γ -∗
-    ∃ future, txn_proph γ future ∗ txnsys_inv_no_future γ future.
+  Lemma txnsys_inv_extract_future γ p :
+    txnsys_inv γ p -∗
+    ∃ future, txn_proph γ p future ∗ txnsys_inv_no_future γ future.
   Proof. iIntros "Htxn". iNamed "Htxn". iFrame "∗ # %". Qed.
 
-  Definition txnsys_inv_with_future_no_ts γ future ts : iProp Σ :=
-    ∃ (tids : gset nat) (past : list action)
-      (tmodcs : gmap nat dbmap) (tmodas : gmap nat tcform) (posts : gmap nat (dbmap -> Prop))
+  Lemma txnsys_inv_merge_future γ p future :
+    txn_proph γ p future -∗
+    txnsys_inv_no_future γ future -∗
+    txnsys_inv γ p.
+  Proof. iIntros "Hproph Htxn". iNamed "Htxn". iFrame "∗ # %". Qed.
+
+  Definition txnsys_inv_with_future_no_ts γ p future ts : iProp Σ :=
+    ∃ (tids tidas : gset nat) (past : list action)
+      (tmods tmodcs : gmap nat dbmap) (tmodas : gmap nat tcform) (posts : gmap nat (dbmap -> Prop))
       (resm : gmap nat txnres) (wrsm : gmap nat (option dbmap)),
       (* witnesses of txn linearization *)
       "Htxnsl" ∷ txns_lnrz_auth γ tids ∗
       (* exclusive transaction IDs *)
       "Hexcl" ∷ tids_excl_auth γ tids ∗
       "Hpart" ∷ partitioned_tids γ tids tmodcs tmodas resm ∗
+      (* transactions predicted to commit *)
+      "Htidcs" ∷ txns_cmt_auth γ tmods ∗
+      (* transactions predicted to abort *)
+      "Htidas" ∷ txns_abt_auth γ tidas ∗
       (* transaction post-conditions *)
       "Hpost" ∷ txnpost_auth γ posts ∗
+      (* prophecy variable *)
+      "Hproph" ∷ txn_proph γ p future ∗
       (* transaction result map *)
       "Hresm" ∷ txnres_auth γ resm ∗
       (* transaction write set map *)
@@ -321,6 +412,9 @@ Section inv.
       (* past action witnesses *)
       "#Hpas" ∷ ([∗ list] a ∈ past, past_action_witness γ a) ∗
       "%Htsge" ∷ ⌜ge_all ts tids⌝ ∗
+      "%Hintids" ∷ ⌜dom tmods ⊆ tids ∧ tidas ⊆ tids⌝ ∗
+      "%Htidcs" ∷ ⌜map_Forall (λ t m, tmodcs !! t = Some m ∨ resm !! t = Some (ResCommitted m)) tmods⌝ ∗
+      "%Htidas" ∷ ⌜dom tmodas = tidas⌝ ∗
       "%Hdomq" ∷ ⌜dom posts = tids⌝ ∗
       "%Hdomw" ∷ ⌜dom wrsm = tids⌝ ∗
       "%Hcmtxn" ∷ ⌜cmtxn_in_past past resm⌝ ∗
@@ -329,9 +423,9 @@ Section inv.
       "%Hcf"   ∷ ⌜conflict_free future tmodcs⌝ ∗
       "%Hcp"   ∷ ⌜conflict_past past future tmodas⌝.
 
-  Lemma txnsys_inv_expose_future_extract_ts γ :
-    txnsys_inv γ -∗
-    ∃ future ts, txnsys_inv_with_future_no_ts γ future ts ∗ ts_auth γ ts.
+  Lemma txnsys_inv_expose_future_extract_ts γ p :
+    txnsys_inv γ p -∗
+    ∃ future ts, txnsys_inv_with_future_no_ts γ p future ts ∗ ts_auth γ ts.
   Proof. iIntros "Htxn". iNamed "Htxn". iFrame "∗ # %". Qed.
 
 End inv.
