src/program_proof/rsm/distx/program/txn.v
@@ -1,6 +1,7 @@
 From Perennial.program_proof.rsm.distx Require Import prelude.
 From Perennial.program_proof.rsm.distx.program Require Import replica_group.
-From Perennial.program_proof.rsm.distx.invariance Require Import linearize.
+From Perennial.program_proof.rsm.distx.invariance Require Import
+  linearize commit preprepare.
 From Goose.github_com.mit_pdos.rsm Require Import distx.
 
 Section program.
@@ -19,18 +20,70 @@ Section program.
     ⊢ |==> ∃ τ, txnmap_auth τ m ∗ ([∗ map] k ↦ v ∈ m, txnmap_ptsto τ k v).
   Admitted.
 
-  Definition own_txn_uninit (txn : loc) (γ : distx_names) : iProp Σ.
+  Lemma txnmap_subseteq τ m1 m2 :
+    txnmap_auth τ m1 -∗
+    txnmap_ptstos τ m2 -∗
+    ⌜m2 ⊆ m1⌝.
   Admitted.
 
-  Definition own_txn_init (txn : loc) (tid : nat) (γ : distx_names) : iProp Σ.
+  (*@ type Txn struct {                                                       @*)
+  (*@     // Transaction timestamp.                                           @*)
+  (*@     ts   uint64                                                         @*)
+  (*@     // Replica groups.                                                  @*)
+  (*@     rgs  map[uint64]*ReplicaGroup                                       @*)
+  (*@     // Buffered write-set.                                              @*)
+  (*@     wrs  map[uint64]map[string]Value                                    @*)
+  (*@     // Participant group of this transaction. Initialized in prepare time. @*)
+  (*@     ptgs []uint64                                                       @*)
+  (*@     // Global prophecy variable (for verification purpose).             @*)
+  (*@     proph primitive.ProphId                                             @*)
+  (*@ }                                                                       @*)
+  Definition own_sharded_wrs (wrsP : loc) (wrs : dbmap) : iProp Σ.
   Admitted.
 
-  (* TODO: we didn't expose [view] as in vMVCC, is that an issue? *)
-  Definition own_txn (txn : loc) (tid : nat) (γ : distx_names) (τ : gname) : iProp Σ.
-  Admitted.
+  Definition own_txn_impl txn (tid : nat) (wrs : dbmap) (proph : proph_id) : iProp Σ :=
+    ∃ (tsW : u64) (rgsP : loc) (wrsP : loc) (ptgsS : Slice.t),
+      "HtsW"     ∷ txn ↦[Txn :: "ts"] #tsW ∗
+      "HrgsP"    ∷ txn ↦[Txn :: "rgs"] #rgsP ∗
+      "HwrsP"    ∷ txn ↦[Txn :: "wrs"] #wrsP ∗
+      "Hwrs"     ∷ own_sharded_wrs wrsP wrs ∗
+      "HptgsS"   ∷ txn ↦[Txn :: "ptgs"] (to_val ptgsS) ∗
+      "HprophP"  ∷ txn ↦[Txn :: "proph"] #proph ∗
+      "%Htsword" ∷ ⌜uint.nat tsW = tid⌝.
 
-  Definition own_txn_ready_ptgs (txn : loc) (tid : nat) (γ : distx_names) (τ : gname) : iProp Σ.
-  Admitted.
+  Definition own_txn_init txn tid γ : iProp Σ :=
+    ∃ proph,
+      "#Hinv" ∷ know_distx_inv γ proph ∗
+      "Htxn"  ∷ own_txn_impl txn tid ∅ proph ∗
+      "%Hvts" ∷ ⌜valid_ts tid⌝.
+
+  Definition own_txn_uninit txn γ : iProp Σ :=
+    ∃ tid, own_txn_init txn tid γ.
+
+  Definition own_txn txn tid rds γ τ : iProp Σ :=
+    ∃ proph wrs,
+      "#Hinv"   ∷ know_distx_inv γ proph ∗
+      "#Hlnrz"  ∷ ([∗ map] key ↦ value ∈ rds, hist_lnrz_at γ key (pred tid) value) ∗
+      "Htxnmap" ∷ txnmap_auth τ (wrs ∪ rds) ∗
+      "Htxn"    ∷ own_txn_impl txn tid wrs proph ∗
+      "%Hincl"  ∷ ⌜dom wrs ⊆ dom rds⌝ ∗
+      "%Hvts"   ∷ ⌜valid_ts tid⌝ ∗
+      "%Hvwrs"  ∷ ⌜valid_wrs wrs⌝.
+
+  Definition own_txn_stable txn tid rds wrs γ τ : iProp Σ :=
+    ∃ proph,
+      "#Hinv"    ∷ know_distx_inv γ proph ∗
+      "#Hlnrz"   ∷ ([∗ map] key ↦ value ∈ rds, hist_lnrz_at γ key (pred tid) value) ∗
+      "#Htxnwrs" ∷ txnwrs_receipt γ tid wrs ∗
+      "Htxnmap"  ∷ txnmap_auth τ (wrs ∪ rds) ∗
+      "Htxn"     ∷ own_txn_impl txn tid wrs proph ∗
+      "%Hincl"  ∷ ⌜dom wrs ⊆ dom rds⌝ ∗
+      "%Hvts"    ∷ ⌜valid_ts tid⌝ ∗
+      "%Hvwrs"   ∷ ⌜valid_wrs wrs⌝.
+
+  Definition own_txn_prepared txn tid rds wrs γ τ : iProp Σ :=
+    (* TODO: something about [ptgs] *)
+    "Htxn" ∷ own_txn_stable txn tid rds wrs γ τ.
 
   Theorem wp_KeyToGroup (key : string) :
     {{{ True }}}
@@ -43,10 +96,10 @@ Section program.
     (*@ }                                                                       @*)
   Admitted.
 
-  Theorem wp_Txn__Read (txn : loc) (tid : nat) (key : string) (value : dbval) γ τ :
-    {{{ own_txn txn tid γ τ ∗ txnmap_ptsto τ key value }}}
+  Theorem wp_Txn__Read txn tid key value rds γ τ :
+    {{{ own_txn txn tid rds γ τ ∗ txnmap_ptsto τ key value }}}
       Txn__Read #txn #(LitString key)
-    {{{ RET (dbval_to_val value); own_txn txn tid γ τ ∗ txnmap_ptsto τ key value }}}.
+    {{{ RET (dbval_to_val value); own_txn txn tid rds γ τ ∗ txnmap_ptsto τ key value }}}.
   Proof.
     (*@ func (txn *Txn) Read(key string) Value {                                @*)
     (*@     gid := KeyToGroup(key)                                              @*)
@@ -63,10 +116,10 @@ Section program.
     (*@ }                                                                       @*)
   Admitted.
 
-  Theorem wp_Txn__Write (txn : loc) (tid : nat) (key : string) (value : string) γ τ :
-    {{{ own_txn txn tid γ τ ∗ (∃ vprev, txnmap_ptsto τ key vprev) }}}
+  Theorem wp_Txn__Write txn tid key value rds γ τ :
+    {{{ own_txn txn tid rds γ τ ∗ (∃ vprev, txnmap_ptsto τ key vprev) }}}
       Txn__Write #txn #(LitString key) #(LitString value)
-    {{{ RET #(); own_txn txn tid γ τ ∗ txnmap_ptsto τ key (Some value) }}}.
+    {{{ RET #(); own_txn txn tid rds γ τ ∗ txnmap_ptsto τ key (Some value) }}}.
   Proof.
     (*@ func (txn *Txn) Write(key string, value string) {                       @*)
     (*@     gid := KeyToGroup(key)                                              @*)
@@ -79,10 +132,10 @@ Section program.
     (*@ }                                                                       @*)
   Admitted.
 
-  Theorem wp_Txn__Delete (txn : loc) (tid : nat) (key : string) (value : dbval) γ τ :
-    {{{ own_txn txn tid γ τ ∗ txnmap_ptsto τ key value }}}
+  Theorem wp_Txn__Delete txn tid key value rds γ τ :
+    {{{ own_txn txn tid rds γ τ ∗ txnmap_ptsto τ key value }}}
       Txn__Delete #txn #(LitString key)
-    {{{ RET #(); own_txn txn tid γ τ ∗ txnmap_ptsto τ key None }}}.
+    {{{ RET #(); own_txn txn tid rds γ τ ∗ txnmap_ptsto τ key None }}}.
   Proof.
     (*@ func (txn *Txn) Delete(key string) {                                    @*)
     (*@     gid := KeyToGroup(key)                                              @*)
@@ -91,44 +144,6 @@ Section program.
     (*@         b : false,                                                      @*)
     (*@     }                                                                   @*)
     (*@     pwrs[key] = v                                                       @*)
-    (*@ }                                                                       @*)
-  Admitted.
-
-  Theorem wp_Txn__abort (txn : loc) (tid : nat) (γ : distx_names) (τ : gname) :
-    txnres_abt γ tid -∗
-    {{{ own_txn txn tid γ τ }}}
-      Txn__abort #txn
-    {{{ RET #(); own_txn_uninit txn γ }}}.
-  Proof.
-    (*@ func (txn *Txn) abort() {                                               @*)
-    (*@     for _, gid := range(txn.ptgs) {                                     @*)
-    (*@         rg := txn.rgs[gid]                                              @*)
-    (*@         pwrs := txn.wrs[gid]                                            @*)
-    (*@                                                                         @*)
-    (*@         // Should abort in parallel.                                    @*)
-    (*@         if uint64(len(pwrs)) != 0 {                                     @*)
-    (*@             rg.Abort(txn.ts)                                            @*)
-    (*@         }                                                               @*)
-    (*@     }                                                                   @*)
-    (*@ }                                                                       @*)
-  Admitted.
-
-  Theorem wp_Txn__commit (txn : loc) (tid : nat) (wrs : dbmap) γ τ :
-    txnres_cmt γ tid wrs -∗
-    {{{ own_txn txn tid γ τ }}}
-      Txn__commit #txn
-    {{{ RET #(); own_txn_uninit txn γ }}}.
-  Proof.
-    (*@ func (txn *Txn) commit() {                                              @*)
-    (*@     for _, gid := range(txn.ptgs) {                                     @*)
-    (*@         rg := txn.rgs[gid]                                              @*)
-    (*@         pwrs := txn.wrs[gid]                                            @*)
-    (*@                                                                         @*)
-    (*@         // Should commit in parallel.                                   @*)
-    (*@         if uint64(len(pwrs)) != 0 {                                     @*)
-    (*@             rg.Commit(txn.ts)                                           @*)
-    (*@         }                                                               @*)
-    (*@     }                                                                   @*)
     (*@ }                                                                       @*)
   Admitted.
 
@@ -146,10 +161,10 @@ Section program.
     (*@ }                                                                       @*)
   Admitted.
 
-  Theorem wp_Txn__setptgs txn tid γ τ :
-    {{{ own_txn txn tid γ τ }}}
+  Theorem wp_Txn__setptgs txn tid rds wrs γ τ :
+    {{{ own_txn txn tid rds γ τ }}}
       Txn__setptgs #txn
-    {{{ RET #(); own_txn_ready_ptgs txn tid γ τ }}}.
+    {{{ RET #(); own_txn_prepared txn tid rds wrs γ τ }}}.
   Proof.
     (*@ func (txn *Txn) setptgs() {                                             @*)
     (*@     var ptgs []uint64 = make([]uint64, 0)                               @*)
@@ -170,16 +185,23 @@ Section program.
     | StAborted => txnres_abt γ ts
     end.
 
-  Theorem wp_Txn__prepare txn tid γ τ :
-    {{{ own_txn txn tid γ τ }}}
+  Theorem wp_Txn__prepare txn tid rds wrs γ τ :
+    {{{ own_txn_stable txn tid rds wrs γ τ }}}
       Txn__prepare #txn
     {{{ (status : txnst), RET #(txnst_to_u64 status);
-        own_txn_ready_ptgs txn tid γ τ ∗ groups_txnst γ tid status
+        own_txn_prepared txn tid rds wrs γ τ ∗ groups_txnst γ tid status
     }}}.
   Proof.
+    iIntros (Φ) "Htxn HΦ".
+    wp_rec.
+
     (*@ func (txn *Txn) prepare() uint64 {                                      @*)
     (*@     var status = TXN_PREPARED                                           @*)
     (*@                                                                         @*)
+    wp_apply (wp_ref_to); first by auto.
+    iIntros (statusP) "HstatusP".
+    wp_pures.
+
     (*@     txn.setptgs()                                                       @*)
     (*@                                                                         @*)
     (*@     var i uint64 = 0                                                    @*)
@@ -200,46 +222,509 @@ Section program.
     (*@ }                                                                       @*)
   Admitted.
 
-  Definition spec_body
+  Definition body_spec
     (body : val) (txn : loc) tid r
     (P : dbmap -> Prop) (Q : dbmap -> dbmap -> Prop)
     (Rc : dbmap -> dbmap -> iProp Σ) (Ra : dbmap -> iProp Σ)
     γ τ : iProp Σ :=
     ∀ Φ,
-    own_txn txn tid γ τ ∗ ⌜P r⌝ ∗ txnmap_ptstos τ r -∗
+    own_txn txn tid r γ τ ∗ ⌜P r⌝ ∗ txnmap_ptstos τ r -∗
     (∀ ok : bool,
-       (own_txn txn tid γ τ ∗
+       (own_txn txn tid r γ τ ∗
         if ok
-        then ∃ w, ⌜Q r w ∧ dom w ⊆ dom r⌝ ∗ (Rc r w ∧ Ra r) ∗ txnmap_ptstos τ (w ∪ r)
+        then ∃ w, ⌜Q r w ∧ dom r = dom w⌝ ∗ (Rc r w ∧ Ra r) ∗ txnmap_ptstos τ w
         else Ra r) -∗ Φ #ok) -∗
     WP body #txn {{ v, Φ v }}.
+
+  Lemma wp_ResolveRead γ p (tid : u64) (key : string) (ts : nat) :
+    ⊢ {{{ ⌜uint.nat tid = ts⌝ }}}
+    <<< ∀∀ acs, txn_proph γ p acs >>>
+      ResolveRead #p #tid #(LitString key) @ ∅
+    <<< ∃ acs', ⌜acs = ActRead ts key :: acs'⌝ ∗ txn_proph γ p acs' >>>
+    {{{ RET #(); True }}}.
+  Admitted.
+
+  Lemma wp_ResolveAbort γ p (tid : u64) (ts : nat) :
+    ⊢ {{{ ⌜uint.nat tid = ts⌝ }}}
+    <<< ∀∀ acs, txn_proph γ p acs >>>
+      ResolveAbort #p #tid @ ∅
+    <<< ∃ acs', ⌜acs = ActAbort ts :: acs'⌝ ∗ txn_proph γ p acs' >>>
+    {{{ RET #(); True }}}.
+  Admitted.
+
+  Lemma wp_ResolveCommit
+    γ p (tid : u64) (ts : nat) (wrsP : loc) (wrs : dbmap) :
+    ⊢ {{{ ⌜uint.nat tid = ts⌝ ∗ own_sharded_wrs wrsP wrs }}}
+    <<< ∀∀ acs, txn_proph γ p acs >>>
+      ResolveCommit #p #tid #wrsP @ ∅
+    <<< ∃ acs', ⌜acs = ActCommit ts wrs :: acs'⌝ ∗ txn_proph γ p acs' >>>
+    {{{ RET #(); own_sharded_wrs wrsP wrs }}}.
+  Admitted.
+
+  Theorem wp_Txn__reset (txn : loc) wrsP wrs :
+    {{{ own_sharded_wrs wrsP wrs }}}
+      Txn__reset #txn
+    {{{ RET #(); own_sharded_wrs wrsP ∅ }}}.
+  Proof.
+    (*@ func (txn *Txn) reset() {                                               @*)
+    (*@     // TODO: reset txn.wrs                                              @*)
+    (*@ }                                                                       @*)
+  Admitted.
+
+  Theorem wp_Txn__commit txn tid rds wrsphys wrsproph γ τ :
+    txns_lnrz_receipt γ tid -∗
+    all_prepared γ tid wrsphys -∗
+    {{{ own_txn_prepared txn tid rds wrsphys γ τ ∗ txns_cmt_elem γ tid wrsproph }}}
+      Txn__commit #txn
+    {{{ RET #(); own_txn_uninit txn γ ∗ ⌜wrsphys = wrsproph⌝ }}}.
+  Proof.
+    iIntros "#Hlnrzed #Hprep" (Φ) "!> [Htxn Htidc] HΦ".
+    wp_rec.
+
+    (*@ func (txn *Txn) commit() {                                              @*)
+    (*@     ResolveCommit(txn.proph, txn.ts, txn.wrs)                           @*)
+    (*@                                                                         @*)
+    iDestruct "Htxn" as (proph) "Htxn".
+    do 2 iNamed "Htxn".
+    do 3 wp_loadField.
+    wp_apply (wp_ResolveCommit with "[$Hwrs]"); first done.
+    iInv "Hinv" as "> HinvO" "HinvC".
+    iApply ncfupd_mask_intro; first set_solver.
+    iIntros "Hmask".
+    iNamed "HinvO".
+    iDestruct (txnsys_inv_extract_future with "Htxnsys") as (future) "[Hproph Htxnsys]".
+    iFrame "Hproph".
+    iIntros "(%future' & %Hfuture & Hproph)".
+    iMod (txnsys_inv_commit with "Hlnrzed Hprep Htxnsys Hgroups Hkeys")
+      as "(Htxnsys & Hgroups & Hkeys & #Hcmt)".
+    { by rewrite Hfuture. }
+    iAssert (⌜wrsphys = wrsproph⌝)%I as %Heq.
+    { iNamed "Htxnsys".
+      iDestruct (txnres_lookup with "Hresm Hcmt") as %Hwrsc.
+      iDestruct (elem_of_committed_partitioned_tids with "Hpart") as %[Hnotinwc Hnotinwa].
+      { by eauto. }
+      iDestruct (txns_cmt_lookup with "Htidcs Htidc") as %Htidc.
+      specialize (Htidcs _ _ Htidc). simpl in Htidcs.
+      (* Prove [resm !! tid = Some (ResCommitted wrs)]. *)
+      destruct Htidcs as [Htmodcs | Hresm].
+      { by rewrite not_elem_of_dom Htmodcs in Hnotinwc. }
+      rewrite Hresm in Hwrsc. symmetry in Hwrsc. inv Hwrsc.
+      done.
+    }
+    (* Close the invariant. *)
+    rewrite Hfuture /=.
+    iDestruct (txnsys_inv_merge_future with "Hproph Htxnsys") as "Htxnsys".
+    iMod "Hmask" as "_".
+    iMod ("HinvC" with "[Htxnsys Hkeys Hgroups]") as "_"; first by iFrame.
+    iIntros "!> Hwrs".
+    wp_pures.
+
+    (*@     for _, gid := range(txn.ptgs) {                                     @*)
+    (*@         rg := txn.rgs[gid]                                              @*)
+    (*@         pwrs := txn.wrs[gid]                                            @*)
+    (*@                                                                         @*)
+    (*@         // Should commit in parallel.                                   @*)
+    (*@         if uint64(len(pwrs)) != 0 {                                     @*)
+    (*@             rg.Commit(txn.ts)                                           @*)
+    (*@         }                                                               @*)
+    (*@     }                                                                   @*)
+    (*@                                                                         @*)
+    (*@     txn.reset()                                                         @*)
+    (*@ }                                                                       @*)
+  Admitted.
+
+  Theorem wp_Txn__commit_in_abort_future txn tid rds wrs γ τ :
+    txns_lnrz_receipt γ tid -∗
+    all_prepared γ tid wrs -∗
+    {{{ own_txn_prepared txn tid rds wrs γ τ ∗ txns_abt_elem γ tid }}}
+      Txn__commit #txn
+    {{{ RET #(); False }}}.
+  Proof.
+    iIntros "#Hlnrzed #Hprep" (Φ) "!> [Htxn Hwabt] HΦ".
+    wp_rec.
+
+    (*@ func (txn *Txn) commit() {                                              @*)
+    (*@     ResolveCommit(txn.proph, txn.ts, txn.wrs)                           @*)
+    (*@                                                                         @*)
+    do 2 iNamed "Htxn".
+    do 3 wp_loadField.
+    wp_apply (wp_ResolveCommit with "[$Hwrs]"); first done.
+    iInv "Hinv" as "> HinvO" "HinvC".
+    iApply ncfupd_mask_intro; first set_solver.
+    iIntros "Hmask".
+    iNamed "HinvO".
+    iDestruct (txnsys_inv_extract_future with "Htxnsys") as (future) "[Hproph Htxnsys]".
+    iFrame "Hproph".
+    iIntros "(%future' & %Hfuture & Hproph)".
+    iMod (txnsys_inv_commit with "Hlnrzed Hprep Htxnsys Hgroups Hkeys")
+      as "(Htxnsys & Hgroups & Hkeys & Hcmt)".
+    { by rewrite Hfuture. }
+    (* Obtain contradiction. *)
+    iNamed "Htxnsys".
+    iDestruct (txnres_lookup with "Hresm Hcmt") as %Hcmt.
+    iDestruct (txns_abt_elem_of with "Htidas Hwabt") as %Hwabt.
+    rewrite -Htidas in Hwabt.
+    iDestruct (elem_of_tmodas_partitioned_tids with "Hpart") as %[_ Hnotin].
+    { apply Hwabt. }
+    by specialize (Hnotin _ Hcmt).
+
+    (*@     for _, gid := range(txn.ptgs) {                                     @*)
+    (*@         rg := txn.rgs[gid]                                              @*)
+    (*@         pwrs := txn.wrs[gid]                                            @*)
+    (*@                                                                         @*)
+    (*@         // Should commit in parallel.                                   @*)
+    (*@         if uint64(len(pwrs)) != 0 {                                     @*)
+    (*@             rg.Commit(txn.ts)                                           @*)
+    (*@         }                                                               @*)
+    (*@     }                                                                   @*)
+    (*@                                                                         @*)
+    (*@     txn.reset()                                                         @*)
+    (*@ }                                                                       @*)
+  Qed.
+
+  Lemma txnsys_inv_abort γ tid future :
+    head_abort future tid ->
+    txnres_abt γ tid -∗
+    txns_abt_elem γ tid -∗
+    txnsys_inv_no_future γ future ==∗
+    txnsys_inv_no_future γ (tail future).
+  Proof.
+    iIntros (Hhead) "#Habt Hwabt Htxn".
+    iNamed "Htxn".
+    (* Obtain [tid ∈ dom resm]. *)
+    iDestruct (txnres_lookup with "Hresm Habt") as %Habt.
+    (* Delete [tid] from [txns_abt_auth]. *)
+    iDestruct (txns_abt_elem_of with "Htidas Hwabt") as %Htid.
+    iMod (txns_abt_delete with "Hwabt Htidas") as "Htidas".
+    (* Re-establish [incorrect_wrs_in_fcc]. *)
+    rewrite -Htidas elem_of_dom in Htid.
+    destruct Htid as [form Hform].
+    iDestruct (big_sepM_delete _ _ tid with "Hiwrs") as "[_ Hiwrs']"; first apply Hform.
+    iClear "Hiwrs".
+    (* Re-establish [partitioned_tids]. *)
+    set tmodas' := delete tid tmodas.
+    iAssert (partitioned_tids γ tids tmodcs tmodas' resm)%I with "[Hpart]" as "Hpart".
+    { iNamed "Hpart".
+      rewrite /partitioned_tids dom_delete_L.
+      rewrite (big_sepS_delete _ (dom tmodas) tid); last first.
+      { by apply elem_of_dom. }
+      iDestruct "Hwabts" as "[_ Hwabts]".
+      iFrame.
+      iPureIntro.
+      intros tidx Htidx.
+      specialize (Hfate _ Htidx). simpl in Hfate.
+      clear -Hfate Habt.
+      apply elem_of_dom_2 in Habt.
+      destruct (decide (tidx = tid)) as [-> | Hne]; set_solver.
+    }
+    iFrame "∗ # %".
+    iPureIntro.
+    split; first set_solver.
+    split; first set_solver.
+    split.
+    { intros tsx wrsx Hwrsx.
+      specialize (Hcf _ _ Hwrsx). simpl in Hcf.
+      by unshelve eapply (first_commit_compatible_inv_tail_future _ _ _ _ _ Hhead).
+    }
+    intros tsx formx Hformx.
+    destruct (decide (tsx = tid)) as [-> | Hne].
+    { by rewrite lookup_delete in Hformx. }
+    rewrite lookup_delete_ne in Hformx; last done.
+    specialize (Hcp _ _ Hformx). simpl in Hcp.
+    rewrite /conflict_cases in Hcp *.
+    destruct formx as [| | wrs | wrs].
+    - by apply no_commit_abort_inv_tail_future.
+    - unshelve eapply (first_abort_inv_tail_future _ _ _ _ Hhead Hcp). inv 1.
+    - apply (first_commit_incompatible_inv_tail_future _ _ _ _ _ Hhead Hcp).
+    - by unshelve eapply (first_commit_compatible_inv_tail_future _ _ _ _ _ Hhead).
+  Qed.
+
+  Theorem wp_Txn__abort txn tid rds wrs γ τ :
+    txnres_abt γ tid -∗
+    {{{ own_txn_prepared txn tid rds wrs γ τ ∗ txns_abt_elem γ tid }}}
+      Txn__abort #txn
+    {{{ RET #(); own_txn_uninit txn γ }}}.
+  Proof.
+    iIntros "#Habt" (Φ) "!> [Htxn Hwabt] HΦ".
+    wp_rec.
+
+    (*@ func (txn *Txn) abort() {                                               @*)
+    (*@     ResolveAbort(txn.proph, txn.ts)                                     @*)
+    (*@                                                                         @*)
+    do 2 iNamed "Htxn".
+    do 2 wp_loadField.
+    wp_apply (wp_ResolveAbort); first done.
+    iInv "Hinv" as "> HinvO" "HinvC".
+    iApply ncfupd_mask_intro; first set_solver.
+    iIntros "Hmask".
+    iNamed "HinvO".
+    iDestruct (txnsys_inv_extract_future with "Htxnsys") as (future) "[Hproph Htxnsys]".
+    iFrame "Hproph".
+    iIntros "(%future' & %Hfuture & Hproph)".
+    iMod (txnsys_inv_abort with "Habt Hwabt Htxnsys") as "Htxnsys".
+    { by rewrite Hfuture. }
+    rewrite Hfuture /=.
+    iDestruct (txnsys_inv_merge_future with "Hproph Htxnsys") as "Htxnsys".
+    iMod "Hmask" as "_".
+    iMod ("HinvC" with "[Htxnsys Hkeys Hgroups]") as "_"; first by iFrame.
+    iIntros "!> _".
+    wp_pures.
+
+    (*@     for _, gid := range(txn.ptgs) {                                     @*)
+    (*@         rg := txn.rgs[gid]                                              @*)
+    (*@         pwrs := txn.wrs[gid]                                            @*)
+    (*@                                                                         @*)
+    (*@         // Should abort in parallel.                                    @*)
+    (*@         if uint64(len(pwrs)) != 0 {                                     @*)
+    (*@             rg.Abort(txn.ts)                                            @*)
+    (*@         }                                                               @*)
+    (*@     }                                                                   @*)
+    (*@                                                                         @*)
+    (*@     txn.reset()                                                         @*)
+    (*@ }                                                                       @*)
+  Admitted.
+
+  Theorem wp_Txn__abort_in_commit_future txn tid rds wrsphys wrsproph γ τ :
+    txnres_abt γ tid -∗
+    {{{ own_txn_prepared txn tid rds wrsphys γ τ ∗ txns_cmt_elem γ tid wrsproph }}}
+      Txn__abort #txn
+    {{{ RET #(); False }}}.
+  Proof.
+    iIntros "#Habt" (Φ) "!> [Htxn Htidc] HΦ".
+    wp_rec.
+
+    (*@ func (txn *Txn) abort() {                                               @*)
+    (*@     ResolveAbort(txn.proph, txn.ts)                                     @*)
+    (*@                                                                         @*)
+    do 2 iNamed "Htxn".
+    do 2 wp_loadField.
+    wp_apply (wp_ResolveAbort); first done.
+    iInv "Hinv" as "> HinvO" "HinvC".
+    iApply ncfupd_mask_intro; first set_solver.
+    iIntros "Hmask".
+    iNamed "HinvO". iNamed "Htxnsys".
+    iFrame "Hproph".
+    iIntros "(%future' & %Hfuture & Hproph)".
+    (* Prove [tid] must not have committed. *)
+    iDestruct (txnres_lookup with "Hresm Habt") as %Habt.
+    iDestruct (txns_cmt_lookup with "Htidcs Htidc") as %Htidc.
+    specialize (Htidcs _ _ Htidc). simpl in Htidcs.
+    destruct Htidcs as [Hwc | Hcmt]; last first.
+    { by rewrite Hcmt in Habt. }
+    specialize (Hcf _ _ Hwc). simpl in Hcf.
+    destruct Hcf as (lp & ls & Hfc & _).
+    assert (Hhead : head_abort future tid).
+    { by rewrite Hfuture. }
+    destruct (first_commit_head_abort _ _ _ _ _ Hfc Hhead) as [].
+  Qed.
+
+  Lemma txnsys_inv_cancel γ tid future :
+    head_abort future tid ->
+    txns_abt_elem γ tid -∗
+    txnwrs_excl γ tid -∗
+    txnsys_inv_no_future γ future ==∗
+    txnsys_inv_no_future γ (tail future).
+  Proof.
+    iIntros (Hhead) "Hwabt Hwrsexcl Htxn".
+    iNamed "Htxn".
+    (* Delete [tid] from [txns_abt_auth]. *)
+    iDestruct (txns_abt_elem_of with "Htidas Hwabt") as %Htid.
+    iMod (txns_abt_delete with "Hwabt Htidas") as "Htidas".
+    (* Insert [(tid, ResAborted)] into [txnres_auth]. *)
+    iDestruct (elem_of_tmodas_partitioned_tids _ _ _ _ _ tid with "Hpart") as %Hnotin.
+    { by rewrite Htidas. }
+    assert (Hresm : resm !! tid = None ∨ resm !! tid = Some ResAborted).
+    { destruct (resm !! tid) as [res |] eqn:Hres; last by left.
+      right.
+      destruct res as [wrs |] eqn:Hwrs.
+      { destruct Hnotin as [_ Hnotin]. by specialize (Hnotin wrs). }
+      done.
+    }
+    set resm' := <[tid := ResAborted]> resm.
+    iAssert (|==> txnres_auth γ resm')%I with "[Hresm]" as "Hresm".
+    { subst resm'.
+      destruct Hresm as [Hnone | Hwabt]; last by rewrite insert_id.
+      by iApply (txnres_insert with "Hresm").
+    }
+    iMod "Hresm" as "Hresm".
+    (* Re-establish [incorrect_wrs_in_fcc]. *)
+    rewrite -Htidas elem_of_dom in Htid.
+    destruct Htid as [form Hform].
+    iDestruct (big_sepM_delete _ _ tid with "Hiwrs") as "[_ Hiwrs']"; first apply Hform.
+    iClear "Hiwrs".
+    (* Persist the txn write-set resource. *)
+    iMod (txnwrs_excl_persist with "Hwrsexcl") as "Hccl".
+    (* Re-establish [valid_res]. *)
+    iDestruct (big_sepM_insert_2 _ _ tid ResAborted with "[Hccl] Hvr") as "#Hvr'".
+    { iFrame. }
+    iClear "Hvr".
+    set tmodas' := delete tid tmodas.
+    (* Re-establish [partitioned_tids]. *)
+    iAssert (partitioned_tids γ tids tmodcs tmodas' resm')%I with "[Hpart]" as "Hpart".
+    { iNamed "Hpart".
+      rewrite /partitioned_tids dom_delete_L.
+      rewrite resm_to_tmods_insert_aborted; last apply Hresm.
+      rewrite (big_sepS_delete _ (dom tmodas) tid); last first.
+      { by apply elem_of_dom. }
+      iDestruct "Hwabts" as "[_ Hwabts]".
+      iFrame.
+      iPureIntro.
+      intros tidx Htidx.
+      rewrite dom_insert_L.
+      specialize (Hfate _ Htidx).
+      clear -Hfate.
+      destruct (decide (tidx = tid)) as [-> | Hne]; set_solver.
+    }
+    iFrame "∗ # %".
+    rewrite /cmtxn_in_past resm_to_tmods_insert_aborted; last apply Hresm.
+    iFrame.
+    iPureIntro.
+    split; first set_solver.
+    split.
+    { subst resm'.
+      intros t m Htm.
+      specialize (Htidcs _ _ Htm). simpl in Htidcs.
+      destruct Htidcs as [? | Hresmt]; first by left.
+      right.
+      destruct (decide (t = tid)) as [-> | Hne].
+      { exfalso. rewrite Hresmt in Hresm. by destruct Hresm. }
+      by rewrite lookup_insert_ne.
+    }
+    split; first set_solver.
+    split; first done.
+    split.
+    { intros tsx wrsx Hwrsx.
+      specialize (Hcf _ _ Hwrsx). simpl in Hcf.
+      by unshelve eapply (first_commit_compatible_inv_tail_future _ _ _ _ _ Hhead).
+    }
+    intros tsx formx Hformx.
+    destruct (decide (tsx = tid)) as [-> | Hne].
+    { by rewrite lookup_delete in Hformx. }
+    rewrite lookup_delete_ne in Hformx; last done.
+    specialize (Hcp _ _ Hformx). simpl in Hcp.
+    rewrite /conflict_cases in Hcp *.
+    destruct formx as [| | wrs | wrs].
+    - by apply no_commit_abort_inv_tail_future.
+    - unshelve eapply (first_abort_inv_tail_future _ _ _ _ Hhead Hcp). inv 1.
+    - apply (first_commit_incompatible_inv_tail_future _ _ _ _ _ Hhead Hcp).
+    - by unshelve eapply (first_commit_compatible_inv_tail_future _ _ _ _ _ Hhead).
+  Qed.
+
+  Theorem wp_Txn__cancel txn tid rds γ τ :
+    {{{ own_txn txn tid rds γ τ ∗ txns_abt_elem γ tid ∗ txnwrs_excl γ tid }}}
+      Txn__cancel #txn
+    {{{ RET #(); own_txn_uninit txn γ }}}.
+  Proof.
+    iIntros (Φ) "(Htxn & Habt & Hwrsexcl) HΦ".
+    wp_rec.
+
+    (*@ func (txn *Txn) cancel() {                                              @*)
+    (*@     ResolveAbort(txn.proph, txn.ts)                                     @*)
+    (*@                                                                         @*)
+    do 2 iNamed "Htxn".
+    do 2 wp_loadField.
+    wp_apply (wp_ResolveAbort); first done.
+    iInv "Hinv" as "> HinvO" "HinvC".
+    iApply ncfupd_mask_intro; first set_solver.
+    iIntros "Hmask".
+    iNamed "HinvO".
+    iDestruct (txnsys_inv_extract_future with "Htxnsys") as (future) "[Hproph Htxnsys]".
+    iFrame "Hproph".
+    iIntros "(%future' & %Hfuture & Hproph)".
+    iMod (txnsys_inv_cancel with "Habt Hwrsexcl Htxnsys") as "Htxnsys".
+    { by rewrite Hfuture. }
+    rewrite Hfuture /=.
+    iDestruct (txnsys_inv_merge_future with "Hproph Htxnsys") as "Htxnsys".
+    iMod "Hmask" as "_".
+    iMod ("HinvC" with "[Htxnsys Hkeys Hgroups]") as "_"; first by iFrame.
+    iIntros "!> _".
+
+    (*@     txn.reset()                                                         @*)
+    (*@ }                                                                       @*)
+    wp_apply (wp_Txn__reset with "Hwrs").
+    iIntros "Hwrs".
+    wp_pures.
+    iApply "HΦ".
+    by iFrame "∗ # %".
+  Qed.
+
+  Theorem wp_Txn__cancel_in_commit_future txn tid rds γ τ :
+    {{{ own_txn txn tid rds γ τ ∗ (∃ m, txns_cmt_elem γ tid m) ∗ txnwrs_excl γ tid }}}
+      Txn__cancel #txn
+    {{{ RET #(); False }}}.
+  Proof.
+    iIntros (Φ) "(Htxn & [%m Htidc] & Hwrsexcl) HΦ".
+    wp_rec.
+
+    (*@ func (txn *Txn) cancel() {                                              @*)
+    (*@     ResolveAbort(txn.proph, txn.ts)                                     @*)
+    (*@                                                                         @*)
+    do 2 iNamed "Htxn".
+    do 2 wp_loadField.
+    wp_apply (wp_ResolveAbort); first done.
+    iInv "Hinv" as "> HinvO" "HinvC".
+    iApply ncfupd_mask_intro; first set_solver.
+    iIntros "Hmask".
+    iNamed "HinvO".
+    iNamed "Htxnsys".
+    iFrame "Hproph".
+    iIntros "(%future' & %Hfuture & Hproph)".
+    (* Obtain [tmods !! tid = Some m]. *)
+    iDestruct (txns_cmt_lookup with "Htidcs Htidc") as %Htidc.
+    specialize (Htidcs _ _ Htidc). simpl in Htidcs.
+    (* Prove [resm !! tid = Some (ResCommitted m)] impossible, i.e., [tid] not committed yet. *)
+    destruct Htidcs as [Htmodcs | Hcmt]; last first.
+    { iDestruct (big_sepM_lookup with "Hvr") as "Hvc"; first apply Hcmt.
+      iDestruct "Hvc" as "[Hwrsrcpt _]".
+      (* Contradicting facts:
+       * 1. Txn still owns exclusively the write-set (which is true before prepare).
+       * Represented as [Hwrsexcl] from the precondition.
+       * 2. Txn has set the write-set and given up the ability to change
+       * (which is true after prepare). Represented as [Hwrsrcpt].
+       *)
+      by iDestruct (txnwrs_frag_agree with "Hwrsexcl Hwrsrcpt") as %Hcontra.
+    }
+    (* Obtain [first_commit]. *)
+    specialize (Hcf _ _ Htmodcs). simpl in Hcf.
+    destruct Hcf as (lp & ls & Hfc & _).
+    (* Obtain contradiction from [first_commit] and [head_abort]. *)
+    assert (Hha : head_abort future tid).
+    { by rewrite Hfuture /head_abort /=. }
+    destruct (first_commit_head_abort _ _ _ _ _ Hfc Hha).
+
+    (*@     txn.reset()                                                         @*)
+    (*@ }                                                                       @*)
+  Qed.
 
   Theorem wp_Txn__Run
     txn (body : val)
     (P : dbmap -> Prop) (Q : dbmap -> dbmap -> Prop)
     (Rc : dbmap -> dbmap -> iProp Σ) (Ra : dbmap -> iProp Σ) γ :
     (∀ r w, (Decision (Q r w))) ->
-    know_distx_inv γ -∗
-    {{{ own_txn_uninit txn γ ∗ (∀ tid r τ, spec_body body txn tid r P Q Rc Ra γ τ) }}}
-    <<< ∀∀ (r : dbmap), ⌜P r⌝ ∗ db_ptstos γ r >>>
-      Txn__Run #txn body @ ↑sysNS
-    <<< ∃∃ (ok : bool) (w : dbmap), if ok then ⌜Q r w⌝ ∗ db_ptstos γ (w ∪ r) else db_ptstos γ r >>>
-    {{{ RET #ok; own_txn_uninit txn γ ∗ if ok then Rc r w else Ra r }}}.
+    ⊢ {{{ own_txn_uninit txn γ ∗ (∀ tid r τ, body_spec body txn tid r P Q Rc Ra γ τ) }}}
+      <<< ∀∀ (r : dbmap), ⌜P r ∧ dom r ⊆ keys_all⌝ ∗ db_ptstos γ r >>>
+        Txn__Run #txn body @ ↑sysNS
+      <<< ∃∃ (ok : bool) (w : dbmap), if ok then ⌜Q r w⌝ ∗ db_ptstos γ w else db_ptstos γ r >>>
+      {{{ RET #ok; own_txn_uninit txn γ ∗ if ok then Rc r w else Ra r }}}.
   Proof.
-    iIntros (Hdec) "#Hinv !>".
+    iIntros (Hdec) "!>".
     iIntros (Φ) "[Htxn Hbody] HAU".
     wp_rec. wp_pures.
 
     (*@ func (txn *Txn) Run(body func(txn *Txn) bool) bool {                    @*)
     (*@     txn.begin()                                                         @*)
     (*@                                                                         @*)
-    wp_apply (wp_Txn__begin with "Htxn").
+    iNamed "Htxn".
+    wp_apply (wp_Txn__begin with "[Htxn]").
+    { iFrame "∗ # %". }
+    clear Hvts tid.
     iInv "Hinv" as "> HinvO" "HinvC".
     iMod (ncfupd_mask_subseteq (⊤ ∖ ↑sysNS)) as "Hclose"; first solve_ndisj.
-    iMod "HAU" as (r) "[[%HP Hdbpts] HAUC]".
+    iMod "HAU" as (rds) "[[[%HP %Hdomr] Hdbpts] HAUC]".
     iModIntro.
     iNamed "HinvO".
-    iDestruct (txnsys_inv_expose_future_extract_ts with "Htxn") as (future ts) "[Htxn Hts]".
+    iDestruct (txnsys_inv_expose_future_extract_ts with "Htxnsys")
+      as (future ts) "[Htxnsys Hts]".
     (* Prove [key_inv] are linearizable after [ts]. *)
     iDestruct (keys_inv_before_linearize with "Hkeys Hts") as "[Hkeys Hts]".
     iExists ts.
@@ -248,60 +733,274 @@ Section program.
     iIntros (tid) "[Hts %Htidgt]".
     iDestruct (ts_witness with "Hts") as "#Htidlb".
 
-    (*@     cmt := body(txn)                                                    @*)
-    (*@     if !cmt {                                                           @*)
-    (*@         // This transaction has not really requested to prepare yet, so no @*)
-    (*@         // cleanup tasks are required.                                  @*)
-    (*@         return false                                                    @*)
-    (*@     }                                                                   @*)
-    (*@                                                                         @*)
-    (*@     status := txn.prepare()                                             @*)
-    (*@                                                                         @*)
-    (*@     if status == TXN_COMMITTED {                                        @*)
-    (*@         // A backup coordinator must have committed this transaction, so there's @*)
-    (*@         // nothing we need to do here.                                  @*)
-    (*@         return true                                                     @*)
-    (*@     }                                                                   @*)
-    (*@                                                                         @*)
-    (*@     if status == TXN_ABORTED {                                          @*)
-    (*@         // Ghost action: Abort this transaction.                        @*)
-    (*@         txn.abort()                                                     @*)
-    (*@         return false                                                    @*)
-    (*@     }                                                                   @*)
-    (*@                                                                         @*)
-    (*@     // Ghost action: Commit this transaction.                           @*)
-    (*@     txn.commit()                                                        @*)
-    (*@     return true                                                         @*)
-    (*@ }                                                                       @*)
     pose proof (peek_spec future tid) as Hpeek.
-    destruct (peek future tid).
-    { (* Case: No commit of timestamp [ts] in the future. *)
-      iMod (txnsys_inv_linearize_abort NC Q with "Htidlb Hdbpts Htxn Hkeys")
-        as "(Hdbpts & Htxn & Hkeys & Hwrsexcl & #HQ & #Hlnrzs & #Hlnrzed)".
-      { (* TODO: Prove [dom r ⊆ keys_all]. *) admit. }
+    set form := peek _ _ in Hpeek.
+    set Qr := λ m, Q rds (m ∪ rds) ∧ dom m ⊆ dom rds.
+    destruct (decide (incorrect_fcc Qr form)) as [Hifcc | HQ].
+    { (* Case: Abort branch. *)
+      iMod (txnsys_inv_linearize_abort form Q with "Htidlb Hdbpts Htxnsys Hkeys")
+        as "(Hdbpts & Htxnsys & Hkeys & Htida & Hwrsexcl & #HQ & #Hlnrzs & #Hlnrzed)".
+      { apply Hdomr. }
       { apply Htidgt. }
       { apply Hpeek. }
       { done. }
       (* Choose the will-abort branch. Use [∅] as placeholder. *)
       iMod ("HAUC" $! false ∅ with "Hdbpts") as "HΦ".
       iMod "Hclose" as "_".
-      iMod ("HinvC" with "[Htxn Hkeys Hgroups]") as "_".
-      { admit. }
+      iMod ("HinvC" with "[Hts Htxnsys Hkeys Hgroups]") as "_".
+      { iNamed "Htxnsys". iFrame "∗ # %". }
       (* Allocate transaction local view [txnmap_ptstos τ r]. *)
-      iMod (txnmap_alloc r) as (τ) "[Htxnmap Htxnpts]".
+      iMod (txnmap_alloc rds) as (τ) "[Htxnmap Htxnpts]".
       iIntros "!> Htxn".
-      iAssert (own_txn txn tid γ τ)%I with "[Htxn Htxnmap]" as "Htxn".
-      { admit. }
-      wp_apply ("Hbody" with "[$Htxn $Htxnpts]"); first done.
-      iIntros (cmt) "[Htxn Hpost]".
-      wp_pures.
-      wp_if_destruct.
-      { iApply "HΦ".
-        (* TODO: weaken [own_txn] to [own_txn_uninit]. *)
-        admit.
+      iAssert (own_txn txn tid rds γ τ)%I with "[Htxn Htxnmap]" as "Htxn".
+      { iClear "Hinv". iNamed "Htxn".
+        iExists _, ∅.
+        rewrite map_empty_union.
+        by iFrame "∗ # %".
       }
+
+      (*@     cmt := body(txn)                                                    @*)
+      (*@                                                                         @*)
+      wp_apply ("Hbody" with "[$Htxn $Htxnpts]"); first done.
+      iIntros (cmt) "[Htxn Hpts]".
+
+      (*@     if !cmt {                                                           @*)
+      (*@         // This transaction has not really requested to prepare yet, so no @*)
+      (*@         // cleanup tasks are required.                                  @*)
+      (*@         txn.cancel()                                                    @*)
+      (*@         return false                                                    @*)
+      (*@     }                                                                   @*)
+      (*@                                                                         @*)
+      wp_if_destruct.
+      { wp_apply (wp_Txn__cancel with "[$Htxn $Htida $Hwrsexcl]").
+        iIntros "Htxn".
+        wp_pures.
+        iApply "HΦ".
+        by iFrame.
+      }
+
+      (*@     status := txn.prepare()                                             @*)
+      (*@                                                                         @*)
+      iDestruct "Hpts" as (w) "([%HQ %Hdomw] & [_ HRa] & Hpts)".
+      iAssert (|={⊤}=> ∃ wrst, own_txn_stable txn tid rds wrst γ τ)%I
+        with "[Htxn Hwrsexcl Hpts]" as "Htxn".
+      { iClear "Hinv". iNamed "Htxn".
+        iDestruct (txnmap_subseteq with "Htxnmap Hpts") as %Hsubseteq.
+        unshelve epose proof (subseteq_dom_eq _ _ Hsubseteq _) as Heq.
+        { clear -Hincl Hdomw. set_solver. }
+        subst w.
+        iInv "Hinv" as "> HinvO" "HinvC".
+        iNamed "HinvO".
+        iMod (txnsys_inv_preprepare with "HQ Hwrsexcl Htxnsys") as "[Htxnsys Hwrsrcpt]".
+        { apply Hvts. }
+        { apply Hvwrs. }
+        { done. }
+        iMod ("HinvC" with "[$Htxnsys $Hkeys $Hgroups]") as "_".
+        by iFrame "∗ # %".
+      }
+      iMod "Htxn" as (wrst) "Htxn".
       wp_apply (wp_Txn__prepare with "Htxn").
       iIntros (status) "[Htxn Hstatus]".
-  Admitted.
+
+      (*@     if status == TXN_COMMITTED {                                        @*)
+      (*@         // A backup coordinator must have committed this transaction, so simply @*)
+      (*@         // reset the write-set here.                                    @*)
+      (*@         txn.reset()                                                     @*)
+      (*@         return true                                                     @*)
+      (*@     }                                                                   @*)
+      (*@                                                                         @*)
+      wp_if_destruct.
+      { destruct status eqn:Hstatus; [done | | done]. clear Heqb.
+        subst status.
+        iDestruct "Hstatus" as (wrs) "Hcmt".
+        (* Obtain a contradiction from [Hcmt] and [Htida]. *)
+        iApply fupd_wp.
+        iInv "Hinv" as "> HinvO" "HinvC".
+        iNamed "HinvO". iNamed "Htxnsys".
+        iDestruct (txnres_lookup with "Hresm Hcmt") as %Hcmt.
+        iDestruct (txns_abt_elem_of with "Htidas Htida") as %Hwabt.
+        rewrite -Htidas in Hwabt.
+        iDestruct (elem_of_tmodas_partitioned_tids with "Hpart") as %[_ Hnotin].
+        { apply Hwabt. }
+        by specialize (Hnotin _ Hcmt).
+      }
+
+      (*@     if status == TXN_ABORTED {                                          @*)
+      (*@         // Ghost action: Abort this transaction.                        @*)
+      (*@         txn.abort()                                                     @*)
+      (*@         return false                                                    @*)
+      (*@     }                                                                   @*)
+      (*@                                                                         @*)
+      wp_if_destruct.
+      { destruct status eqn:Hstatus; [done | done |]. clear Heqb.
+        subst status.
+        wp_apply (wp_Txn__abort with "Hstatus [$Htxn $Htida]").
+        iIntros "Htxn".
+        wp_pures.
+        iApply "HΦ".
+        by iFrame.
+      }
+
+      (*@     // Ghost action: Commit this transaction.                           @*)
+      (*@     txn.commit()                                                        @*)
+      (*@     return true                                                         @*)
+      (*@ }                                                                       @*)
+      destruct status as [wrs | |] eqn:Hstatus; [| done | done]. clear Heqb.
+      subst status. simpl.
+      iAssert (⌜wrst = wrs⌝)%I as %->.
+      { iClear "Hinv". iNamed "Htxn".
+        iDestruct "Hstatus" as "[#Hwrsrcpt _]".
+        by iDestruct (txnwrs_receipt_agree with "Hwrsrcpt Htxnwrs") as %?.
+      }
+      wp_apply (wp_Txn__commit_in_abort_future with "Hlnrzed Hstatus [$Htxn $Htida]").
+      iIntros ([]).
+    }
+    { (* Case: Commit branch. *)
+      destruct form as [| | wrs | wrs]; [done | done | done |].
+      apply dec_stable in HQ. simpl in Hpeek.
+      subst Qr.
+      destruct HQ as [HQ Hdomwrs].
+      iMod (txnsys_inv_linearize_commit wrs Q with "Htidlb Hdbpts Htxnsys Hkeys")
+        as "(Hdbpts & Htxnsys & Hkeys & Htidc & Hwrsexcl & #HQ & #Hlnrzs & #Hlnrzed)".
+      { apply Hdomwrs. }
+      { apply Hdomr. }
+      { apply Htidgt. }
+      { apply Hpeek. }
+      (* Choose the will-commit branch. *)
+      iMod ("HAUC" $! true (wrs ∪ rds) with "[$Hdbpts]") as "HΦ"; first done.
+      iMod "Hclose" as "_".
+      iMod ("HinvC" with "[Hts Htxnsys Hkeys Hgroups]") as "_".
+      { iNamed "Htxnsys". iFrame "∗ # %". }
+      iClear "Hinv". clear proph.
+      (* Allocate transaction local view [txnmap_ptstos τ r]. *)
+      iMod (txnmap_alloc rds) as (τ) "[Htxnmap Htxnpts]".
+      iIntros "!> Htxn".
+      iAssert (own_txn txn tid rds γ τ)%I with "[Htxn Htxnmap]" as "Htxn".
+      { iNamed "Htxn".
+        iExists _, ∅.
+        rewrite map_empty_union.
+        by iFrame "∗ # %".
+      }
+
+      (*@     cmt := body(txn)                                                    @*)
+      (*@                                                                         @*)
+      wp_apply ("Hbody" with "[$Htxn $Htxnpts]"); first done.
+      iIntros (cmt) "[Htxn Hpts]".
+
+      (*@     if !cmt {                                                           @*)
+      (*@         // This transaction has not really requested to prepare yet, so no @*)
+      (*@         // cleanup tasks are required.                                  @*)
+      (*@         txn.cancel()                                                    @*)
+      (*@         return false                                                    @*)
+      (*@     }                                                                   @*)
+      (*@                                                                         @*)
+      wp_if_destruct.
+      { wp_apply (wp_Txn__cancel_in_commit_future with "[$Htxn $Htidc $Hwrsexcl]").
+        iIntros ([]).
+      }
+
+      (*@     status := txn.prepare()                                             @*)
+      (*@                                                                         @*)
+      clear HQ.
+      iDestruct "Hpts" as (w) "([%HQ %Hdomw] & [HRc _] & Hpts)".
+      iAssert (|={⊤}=> ∃ wrst, own_txn_stable txn tid rds wrst γ τ ∗ ⌜w = wrst ∪ rds⌝)%I
+        with "[Htxn Hwrsexcl Hpts]" as "Htxn".
+      { iDestruct "Htxn" as (p wrst) "Htxn". iNamed "Htxn".
+        iDestruct (txnmap_subseteq with "Htxnmap Hpts") as %Hsubseteq.
+        unshelve epose proof (subseteq_dom_eq _ _ Hsubseteq _) as Heq.
+        { clear -Hincl Hdomw. set_solver. }
+        subst w.
+        iInv "Hinv" as "> HinvO" "HinvC".
+        iNamed "HinvO".
+        iMod (txnsys_inv_preprepare with "HQ Hwrsexcl Htxnsys") as "[Htxnsys Hwrsrcpt]".
+        { apply Hvts. }
+        { apply Hvwrs. }
+        { done. }
+        iMod ("HinvC" with "[$Htxnsys $Hkeys $Hgroups]") as "_".
+        by iFrame "∗ # %".
+      }
+      iMod "Htxn" as (wrst) "[Htxn %Heq]". subst w.
+      wp_apply (wp_Txn__prepare with "Htxn").
+      iIntros (status) "[Htxn Hstatus]".
+
+      (*@     if status == TXN_COMMITTED {                                        @*)
+      (*@         // A backup coordinator must have committed this transaction, so simply @*)
+      (*@         // reset the write-set here.                                    @*)
+      (*@         txn.reset()                                                     @*)
+      (*@         return true                                                     @*)
+      (*@     }                                                                   @*)
+      (*@                                                                         @*)
+      wp_if_destruct.
+      { destruct status eqn:Hstatus; [done | | done]. clear Heqb.
+        subst status.
+        iDestruct "Hstatus" as (wrsc) "#Hwrsc".
+        iNamed "Htxn".
+        (* Obtain [wrsc = wrs ∧ wrst = wrs]. *)
+        iAssert (|={⊤}=> txns_cmt_elem γ tid wrs ∗ ⌜wrsc = wrs ∧ wrst = wrs⌝)%I
+          with "[Htidc]" as "Htidc".
+        { iInv "Hinv" as "> HinvO" "HinvC".
+          iNamed "HinvO". iNamed "Htxnsys".
+          iDestruct (txnres_lookup with "Hresm Hwrsc") as %Hwrsc.
+          iDestruct (elem_of_committed_partitioned_tids with "Hpart") as %[Hnotinwc Hnotinwa].
+          { by eauto. }
+          iDestruct (txns_cmt_lookup with "Htidcs Htidc") as %Htidc.
+          apply Htidcs in Htidc.
+          (* Prove [resm !! tid = Some (ResCommitted wrs)]. *)
+          destruct Htidc as [Htmodcs | Hresm].
+          { by rewrite not_elem_of_dom Htmodcs in Hnotinwc. }
+          rewrite Hresm in Hwrsc. symmetry in Hwrsc. inv Hwrsc.
+          iDestruct (big_sepM_lookup with "Hvr") as "Hr"; first apply Hresm.
+          iDestruct "Hr" as "[Hrcp _]".
+          iDestruct (txnwrs_receipt_agree with "Hrcp Htxnwrs") as %->.
+          iMod ("HinvC" with "[-Htidc]") as "_".
+          { by iFrame "∗ # %". }
+          by iFrame "∗ %".
+        }
+        iMod "Htidc" as "[Htidc %Heq]".
+        destruct Heq as [-> ->].
+        iNamed "Htxn".
+        wp_apply (wp_Txn__reset with "Hwrs").
+        iIntros "Hwrs".
+        wp_pures.
+        iApply "HΦ".
+        by iFrame "∗ # %".
+      }
+      rename Heqb into Hstatusnc.
+
+      (*@     if status == TXN_ABORTED {                                          @*)
+      (*@         // Ghost action: Abort this transaction.                        @*)
+      (*@         txn.abort()                                                     @*)
+      (*@         return false                                                    @*)
+      (*@     }                                                                   @*)
+      (*@                                                                         @*)
+      wp_if_destruct.
+      { destruct status eqn:Hstatus; [done | done |]. clear Heqb.
+        subst status. simpl.
+        wp_apply (wp_Txn__abort_in_commit_future with "Hstatus [$Htxn $Htidc]").
+        iIntros ([]).
+      }
+      rename Heqb into Hstatusna.
+
+      (*@     // Ghost action: Commit this transaction.                           @*)
+      (*@     txn.commit()                                                        @*)
+      (*@     return true                                                         @*)
+      (*@ }                                                                       @*)
+      destruct status as [wrsc | |] eqn:Hstatus; [| done | done].
+      clear Hstatusnc Hstatusna.
+      iDestruct "Hstatus" as "#Hprep". simpl.
+      subst status.
+      iAssert (⌜wrsc = wrst⌝)%I as %->.
+      { iNamed "Htxn".
+        iDestruct "Hprep" as "[Hwrsrcpt _]".
+        by iDestruct (txnwrs_receipt_agree with "Htxnwrs Hwrsrcpt") as %?.
+      }
+      wp_apply (wp_Txn__commit with "Hlnrzed Hprep [Htxn Htidc]").
+      { iFrame "∗ #". }
+      iIntros "[Htxn %Heq]". subst wrst.
+      wp_pures.
+      iApply "HΦ".
+      by iFrame.
+    }
+  Qed.
 
 End program.
