src/program_proof/rsm/distx/res.v
@@ -226,11 +226,19 @@ Section res.
   Definition txnwrs_excl γ (ts : nat) :=
     txnwrs_frag γ ts (DfracOwn 1) None.
 
+  Definition txnwrs_cancel γ (ts : nat) :=
+    txnwrs_frag γ ts DfracDiscarded None.
+
   Definition txnwrs_receipt γ (ts : nat) (wrs : dbmap) :=
     txnwrs_frag γ ts DfracDiscarded (Some wrs).
 
   #[global]
-  Instance txnwrs_receipt_persistent γ ts wrs  :
+  Instance txnwrs_cancel_persistent γ ts :
+    Persistent (txnwrs_cancel γ ts).
+  Admitted.
+
+  #[global]
+  Instance txnwrs_receipt_persistent γ ts wrs :
     Persistent (txnwrs_receipt γ ts wrs).
   Admitted.
 
@@ -240,23 +248,33 @@ Section res.
     txnwrs_auth γ (<[ts := None]> wrsm) ∗ txnwrs_excl γ ts.
   Admitted.
 
+  Lemma txnwrs_excl_persist γ ts :
+    txnwrs_excl γ ts ==∗ txnwrs_cancel γ ts.
+  Admitted.
+
   Lemma txnwrs_set γ wrsm ts wrs :
     txnwrs_excl γ ts -∗
     txnwrs_auth γ wrsm ==∗
     txnwrs_auth γ (<[ts := Some wrs]> wrsm) ∗ txnwrs_receipt γ ts wrs.
   Admitted.
 
-  Lemma txnwrs_frag_lookup γ wrsm ts dq owrs :
+  Lemma txnwrs_lookup γ wrsm ts dq owrs :
     txnwrs_frag γ ts dq owrs -∗
     txnwrs_auth γ wrsm -∗
     ⌜wrsm !! ts = Some owrs⌝.
+  Admitted.
+
+  Lemma txnwrs_frag_agree γ ts dq1 dq2 owrs1 owrs2 :
+    txnwrs_frag γ ts dq1 owrs1 -∗
+    txnwrs_frag γ ts dq2 owrs2 -∗
+    ⌜owrs2 = owrs1⌝.
   Admitted.
 
   Lemma txnwrs_receipt_lookup γ wrsm ts wrs :
     txnwrs_receipt γ ts wrs -∗
     txnwrs_auth γ wrsm -∗
     ⌜wrsm !! ts = Some (Some wrs)⌝.
-  Proof. iIntros "#Hwrs Hwrsm". by iApply txnwrs_frag_lookup. Qed.
+  Proof. iIntros "#Hwrs Hwrsm". by iApply txnwrs_lookup. Qed.
 
   Lemma txnwrs_excl_elem_of γ wrsm ts :
     txnwrs_excl γ ts -∗
@@ -264,7 +282,7 @@ Section res.
     ⌜ts ∈ dom wrsm⌝.
   Proof.
     iIntros "Hwrs Hwrsm".
-    iDestruct (txnwrs_frag_lookup with "Hwrs Hwrsm") as %Hlookup.
+    iDestruct (txnwrs_lookup with "Hwrs Hwrsm") as %Hlookup.
     by apply elem_of_dom_2 in Hlookup.
   Qed.
 
@@ -464,6 +482,50 @@ Section res.
     ⌜tid ∈ tids⌝.
   Admitted.
 
+  (* Transactions predicted to abort. *)
+  Definition txns_abt_auth γ (tids : gset nat) : iProp Σ.
+  Admitted.
+
+  Definition txns_abt_elem γ (tid : nat) : iProp Σ.
+  Admitted.
+
+  Lemma txns_abt_insert {γ tids} tid :
+    tid ∉ tids ->
+    txns_abt_auth γ tids ==∗
+    txns_abt_auth γ ({[ tid ]} ∪ tids) ∗ txns_abt_elem γ tid.
+  Admitted.
+
+  Lemma txns_abt_delete {γ tids} tid :
+    txns_abt_elem γ tid -∗
+    txns_abt_auth γ tids ==∗
+    txns_abt_auth γ (tids ∖ {[ tid ]}).
+  Admitted.
+
+  Lemma txns_abt_elem_of γ tids tid :
+    txns_abt_auth γ tids -∗
+    txns_abt_elem γ tid -∗
+    ⌜tid ∈ tids⌝.
+  Admitted.
+
+  (* Transactions predicted to commit/has committed. *)
+  Definition txns_cmt_auth γ (tmods : gmap nat dbmap) : iProp Σ.
+  Admitted.
+
+  Definition txns_cmt_elem γ (tid : nat) (wrs : dbmap) : iProp Σ.
+  Admitted.
+
+  Lemma txns_cmt_insert {γ tmods} tid wrs :
+    tmods !! tid = None ->
+    txns_cmt_auth γ tmods ==∗
+    txns_cmt_auth γ (<[tid := wrs]> tmods) ∗ txns_cmt_elem γ tid wrs.
+  Admitted.
+
+  Lemma txns_cmt_lookup γ tmods tid wrs :
+    txns_cmt_auth γ tmods -∗
+    txns_cmt_elem γ tid wrs -∗
+    ⌜tmods !! tid = Some wrs⌝.
+  Admitted.
+
   (* Exclusive transaction IDs. *)
   Definition tids_excl_auth γ (tids : gset nat) : iProp Σ.
   Admitted.
@@ -618,7 +680,7 @@ Section res.
     Persistent (ts_lb γ ts).
   Admitted.
 
-  Definition txn_proph γ (acts : list action) : iProp Σ.
+  Definition txn_proph γ (p : proph_id) (acts : list action) : iProp Σ.
   Admitted.
 
 End res.
