src/program_proof/rsm/distx/invariance/abort.v
@@ -1,47 +1,7 @@
 From Perennial.program_proof.rsm.distx Require Import prelude.
 
-Lemma resm_to_tmods_insert_aborted resm ts :
-  resm !! ts = None ->
-  resm_to_tmods (<[ts := ResAborted]> resm) = resm_to_tmods resm.
-Proof.
-  intros Hnotin.
-  rewrite /resm_to_tmods omap_insert_None; last done.
-  rewrite delete_notin; first done.
-  by rewrite lookup_omap Hnotin.
-Qed.
-
 Section inv.
   Context `{!distx_ghostG Σ}.
 
-  Lemma txnsys_inv_abort γ ts :
-    some_aborted γ ts -∗
-    txnsys_inv γ ==∗
-    txnsys_inv γ ∗
-    txnres_abt γ ts.
-  Proof.
-    iIntros "#Habt Htxn".
-    iNamed "Htxn".
-    destruct (resm !! ts) as [res |] eqn:Hres; last first.
-    { (* Case: [ts] has neither aborted nor committed yet. *)
-      iMod (txnres_insert ts ResAborted with "Hresm") as "Hresm"; first done.
-      iDestruct (txnres_witness with "Hresm") as "#Hreceipt".
-      { apply lookup_insert. }
-      iFrame "∗ # %".
-      rewrite /partitioned_tids resm_to_tmods_insert_aborted; last done.
-      rewrite big_sepM_insert; last done.
-      iFrame "∗ #".
-      iPureIntro.
-      by rewrite /cmtxn_in_past resm_to_tmods_insert_aborted; last apply Hres.
-    }
-    destruct res as [wrsc |]; last first.
-    { (* Case: [ts] aborted; get a witness without any update. *)
-      iDestruct (txnres_witness with "Hresm") as "#Hreceipt"; first apply Hres.
-      by iFrame "∗ # %".
-    }
-    (* Case: [ts] committed; contradiction. *)
-    iDestruct (big_sepM_lookup with "Hvr") as "#Hprep"; first apply Hres.
-    simpl.
-    iDestruct (all_prepared_some_aborted_false with "Hprep Habt") as %[].
-  Qed.
 
 End inv.
